%%
% Please see https://bitbucket.org/rivanvx/beamer/wiki/Home for obtaining beamer.
%%

\documentclass{beamer}

\usepackage[utf8]{inputenc}


\begin{document}
Beweis f√ºr \textbf{[Lit\_15b]} Satz 12.1 (12.7):

"keine Alterung bei Exponentialverteilung"

\begin{align*}
	\quad & P( \lbrace t < T_B \leq t + \Delta t \rbrace / \lbrace T_B > t \rbrace)\\
	\overset{(12.6)}{=} & \frac{F_{TB}(t + \Delta t) - F_{TB}(t)}{1-F_{TB}(t)} \\
	\overset{(12.4)}{=} & \frac{(1-e^{-\lambda(t + \Delta t)}) - (1-e^{-\lambda t})}{1-(1-e^{-\lambda t})}\\
	= & \frac{1 - e^{-\lambda(t + \Delta t)} - 1 + e^{-\lambda t}}{e^{-\lambda t}} \\
	= & \frac{e^{-\lambda t} - e^{-\lambda(t + \Delta t)}}{e^{-\lambda t}} \\
	= & 1 - \frac{e^{-\lambda(t + \Delta t)}}{e^{-\lambda t}} \\
	= & 1 - e^{-\lambda(t + \Delta t) + \lambda t} \\
	= & 1 - e^{-\lambda t - \lambda \Delta t + \lambda t} \\
	= & 1 - e^{-\lambda \Delta t} \qed
\end{align*}
\end{document}
